Makefile
@@ -32,10 +32,6 @@ lib: CoqMakefile
 	$(MAKE) -f CoqMakefile src/AdversarySafety.vo \
 			       src/ModelCheck/InvariantSearch.vo
 
-por: CoqMakefile
-	$(eval TS := src/ModelCheck/PartialOrderReduction.vo)
-	$(MAKE) -f CoqMakefile pretty-timed TGTS=$(TS)
-
 test: lib
 	$(eval TS := "protocols/Verification/PGPSecure.vo")
 	$(MAKE) -f CoqMakefile pretty-timed TGTS=$(TS)
