README.md
@@ -1,11 +1,40 @@
 # Secure Protocols Implemented CorrectlY (SPICY)
 
-Some witty project description.
+This repository contains the main developments of the SPICY protocol development and specification tool.
+
+## Repository Layout
+
+This repository has three top-level directories:
+* Frap -- we bootstrapped the project by using some developments from the FRAP library
+* src -- core library code, including Domain Specific Languages (DSLs), their semantics, and the safety theorem
+* protocols -- several test protocols proven correct
+
+Some good places to start to get a feel for the formalized languages and main safety result:
+
+* src/IdealWorld.v -- formalization of the Ideal World language.
+* src/RealWorld.v -- formalization of the Real World language.
+* src/Simulation.v -- development of our simulation statements between the Ideal and Real worlds (the actual simulation definitions can be found in the "Simulation" section).
+* src/AdversarySafety.v -- the main theorems and lemmas stating the safety result.
+
+The main safety results within AdversarySafety warrant some further discussion.
+The last theorem (`refines_could_generate`) is the statement that if a Real
+World protocol refines an Ideal World protocol, then traces in the Real World
+can be reproduced in the Ideal World. A few hundred lines up from there, in
+`refines_ok_with_adversary` is the main lemma supporting
+`refines_could_generate` where we show that, starting from a refinement
+condition in a universe with no adversary, we can inject arbitrary adversary
+code and obtain a refinement condition within this new universe.
+
+Using the above library code, we have verified several exemplar protocols.
+
+* protocols/PGP.v (protocol impl) and protocols/Verification/PGPSecure.v (correctness proof) -- describes a secret sharing protocol inspired by the PGP protocol.
+* protocols/SecureDNS.v (protocol impl) and protocols/Verification/SecureDNSSecure.v (correctness proof) -- describes a protocol similar in spirit to (but much simplified) Daniel Bernstein's DNSCurve for encrypted DNS.
+* protocols/AvgSalary.v and protocols/Verification/AvgSalarySecure.v -- describes a simple aggregation service, interesting because it involves more than two parties.
+* protocols/P2P.v and protocols/Verification/P2PSecure.v -- describes a network authentication protocol by a trusted third party showing an alternative way of bootstrapping trusted keys
 
 ## Setup
 
 Setup notes for future me.
-
 
 ### Installing coq
 
@@ -25,22 +54,25 @@ Now, whenever you want to install a new version, just do:
 ```bash
 opam update
 
-opam switch create coq-<ver> ocaml-base-compiler.4.08.1
+opam switch create coq-8.13.2 ocaml-base-compiler.4.11.1
 
-opam install coq.<ver>
-opam pin add coq <ver>
+opam install coq.8.13.2
+opam pin add coq 8.13.2
 ```
 
 ### Compiling Project
 
 ```bash
-git clone ssh://git@github.mit.edu/mitll-crows/key-management-model
-cd key-management-model
+git clone <url>
 
 # Pull in submodules
 git submodule update --init --recursive
 
-make
+# Compiles the faster paper example protocol
+make paper-fast
+
+# Compiles all paper example protocols
+make paper-all
 ```
 
 ## Disclaimer
